Finish NIUtils.v proofs (#1777)
The definition of fresh_han and fresh_chan needed to be changed so
that the labels of unused objects is public. For the other definition
where labels are partially secret, I think this would need to stay
"top". Either way, fresh_han and fresh_chan are not really parts of the
implementation; in the implementation I think these objects are just
genuinely newly created objects.

There is also some leftover fixup that didn't quite make it into the leftover PR.

experimental/ni_coq/vfiles/ModelSemUtils.v
@@ -109,9 +109,15 @@ Definition node_del_rhans (hs: Ensemble handle)(n: node): node :=
 
 Definition new_chan := Some {| ms := [] |}.
 
-Definition fresh_han s h := s.(chans).[?h] = Labeled channel None top.
+Definition fresh_han s h := s.(chans).[?h] = Labeled channel None bot.
 
-Definition fresh_nid s id := s.(nodes).[?id] = Labeled node None top.
+Definition fresh_nid s id := s.(nodes).[?id] = Labeled node None bot.
+
+(* unoccupied handles / IDs are secret for the model + security-def where 
+labels are partially secret *)
+Definition fresh_han_top s h := s.(chans).[?h] = Labeled channel None top.
+
+Definition fresh_nid_top s id := s.(nodes).[?id] = Labeled node None top.
 
 Definition s_set_call s id c :=
     match (s.(nodes).[?id]).(obj) with
